aarch64 refine: introduce pspace_canonical'
It turns out the concept is needed after all in CRefine and is easier
to prove as a separate invariant on the design level than transporting
it down from AInvs via assertions (would not only take too many
assertions, but most of these would be in generic code, polluting the
proofs for other architectures).

The current definition sticks to validity of kernel-virtual addresses,
using canonical_bit, instead of trying to encode stronger properties
such as using the IPA size or physical address size after translation.
This is because the main use of pspace_canonical' is in CRefine, where
we only need the weaker canonical_bit size for kernel pointers.

Signed-off-by: Gerwin Klein <gerwin.klein@proofcraft.systems>

proof/refine/AARCH64/Invariants_H.thy
@@ -439,6 +439,7 @@ where valid_cap'_def:
   | UntypedCap d r n f \<Rightarrow>
       valid_untyped' d r n f s \<and> r \<noteq> 0 \<and> minUntypedSizeBits \<le> n \<and> n \<le> maxUntypedSizeBits
         \<and> f \<le> 2^n \<and> is_aligned (of_nat f :: machine_word) minUntypedSizeBits
+        \<and> canonical_address r
   | EndpointCap r badge x y z t \<Rightarrow> ep_at' r s
   | NotificationCap r badge x y \<Rightarrow> ntfn_at' r s
   | CNodeCap r bits guard guard_sz \<Rightarrow>
@@ -539,6 +540,9 @@ definition
 where
   "pspace_distinct' s \<equiv>
    \<forall>x \<in> dom (ksPSpace s). ps_clear x (objBitsKO (the (ksPSpace s x))) s"
+
+definition pspace_canonical' :: "kernel_state \<Rightarrow> bool" where
+  "pspace_canonical' s \<equiv> \<forall>p \<in> dom (ksPSpace s). canonical_address p"
 
 definition
   valid_objs' :: "kernel_state \<Rightarrow> bool"
@@ -802,6 +806,7 @@ definition
 where
   "valid_pspace' \<equiv> valid_objs' and
                    pspace_aligned' and
+                   pspace_canonical' and
                    pspace_distinct' and
                    no_0_obj' and
                    valid_mdb'"
@@ -1670,7 +1675,7 @@ lemmas valid_irq_states'_def = valid_irq_masks'_def
 
 lemma valid_pspaceE' [elim]:
   "\<lbrakk>valid_pspace' s;
-    \<lbrakk> valid_objs' s; pspace_aligned' s; pspace_distinct' s; no_0_obj' s;
+    \<lbrakk> valid_objs' s; pspace_aligned' s; pspace_distinct' s; pspace_canonical' s; no_0_obj' s;
       valid_mdb' s \<rbrakk> \<Longrightarrow> R \<rbrakk> \<Longrightarrow> R"
   unfolding valid_pspace'_def by simp
 
@@ -1788,7 +1793,7 @@ lemma valid_pspace':
   "valid_pspace' s \<Longrightarrow> ksPSpace s = ksPSpace s' \<Longrightarrow> valid_pspace' s'"
   by  (auto simp add: valid_pspace'_def valid_objs'_def pspace_aligned'_def
                      pspace_distinct'_def ps_clear_def no_0_obj'_def ko_wp_at'_def
-                     typ_at'_def
+                     typ_at'_def pspace_canonical'_def
            intro: valid_obj'_pspaceI valid_mdb'_pspaceI)
 
 lemma ex_cte_cap_to_pspaceI'[elim]:
@@ -2637,6 +2642,10 @@ lemma pspace_distinct_update [iff]:
   "pspace_distinct' (f s) = pspace_distinct' s"
   by (simp add: pspace pspace_distinct'_def ps_clear_def)
 
+lemma pspace_canonical_update [iff]:
+  "pspace_canonical' (f s) = pspace_canonical' s"
+  by (simp add: pspace pspace_canonical'_def ps_clear_def)
+
 lemma pred_tcb_at_update [iff]:
   "pred_tcb_at' proj P p (f s) = pred_tcb_at' proj P p s"
   by (simp add: pred_tcb_at'_def)
@@ -3236,6 +3245,14 @@ lemma invs_valid_global'[elim!]:
   "invs' s \<Longrightarrow> valid_global_refs' s"
   by (fastforce simp: invs'_def valid_state'_def)
 
+lemma invs_pspace_canonical'[elim!]:
+  "invs' s \<Longrightarrow> pspace_canonical' s"
+  by (fastforce dest!: invs_valid_pspace' simp: valid_pspace'_def)
+
+lemma valid_pspace_canonical'[elim!]:
+  "valid_pspace' s \<Longrightarrow> pspace_canonical' s"
+  by (rule valid_pspaceE')
+
 lemma invs'_invs_no_cicd:
   "invs' s \<Longrightarrow> all_invs_but_ct_idle_or_in_cur_domain' s"
   by (simp add: invs'_to_invs_no_cicd'_def)
@@ -3337,6 +3354,59 @@ lemma mask_wordRadix_less_wordBits:
 lemma priority_mask_wordRadix_size:
   "unat ((w::priority) && mask wordRadix) < wordBits"
   by (rule mask_wordRadix_less_wordBits, simp add: wordRadix_def word_size)
+
+lemma canonical_address_mask_eq:
+  "canonical_address p = (p && mask (Suc canonical_bit) = p)"
+  by (simp add: canonical_address_def canonical_address_of_def ucast_ucast_mask canonical_bit_def)
+
+lemma canonical_address_and:
+  "canonical_address p \<Longrightarrow> canonical_address (p && b)"
+  by (simp add: canonical_address_range word_and_le)
+
+lemma canonical_address_add:
+  assumes "is_aligned p n"
+  assumes "f < 2 ^ n"
+  assumes "n \<le> canonical_bit"
+  assumes "canonical_address p"
+  shows "canonical_address (p + f)"
+proof -
+  from `f < 2 ^ n`
+  have "f \<le> mask n"
+    by (simp add: mask_plus_1 plus_one_helper)
+
+  from `canonical_address p`
+  have "p && mask (Suc canonical_bit) = p"
+    by (simp add: canonical_address_mask_eq)
+  moreover
+  from `f \<le> mask n` `is_aligned p n`
+  have "p + f = p || f"
+    by (simp add: word_and_or_mask_aligned)
+  moreover
+  from `f \<le> mask n` `n \<le> canonical_bit`
+  have "f \<le> mask (Suc canonical_bit)"
+    using le_smaller_mask by fastforce
+  hence "f && mask (Suc canonical_bit) = f"
+    by (simp add: le_mask_imp_and_mask)
+  ultimately
+  have "(p + f) && mask (Suc canonical_bit) = p + f"
+    by (simp add: word_ao_dist)
+  thus ?thesis
+    by (simp add: canonical_address_mask_eq)
+qed
+
+lemma range_cover_canonical_address:
+  "\<lbrakk> range_cover ptr sz us n ; p < n ;
+     canonical_address (ptr && ~~ mask sz) ; sz \<le> maxUntypedSizeBits \<rbrakk>
+   \<Longrightarrow> canonical_address (ptr + of_nat p * 2 ^ us)"
+  apply (subst word_plus_and_or_coroll2[symmetric, where w = "mask sz"])
+  apply (subst add.commute)
+  apply (subst add.assoc)
+  apply (rule canonical_address_add[where n=sz] ; simp add: untypedBits_defs is_aligned_neg_mask)
+   apply (drule (1) range_cover.range_cover_compare)
+   apply (clarsimp simp: word_less_nat_alt)
+   apply unat_arith
+  apply (simp add: canonical_bit_def)
+  done
 
 end
 (* The normalise_obj_at' tactic was designed to simplify situations similar to:
