proof/refine/AARCH64/Detype_R.thy
@@ -751,6 +751,7 @@ context delete_locale begin interpretation Arch . (*FIXME: arch_split*)
 
 lemma valid_objs: "valid_objs' s"
   and        pa: "pspace_aligned' s"
+  and        pc: "pspace_canonical' s"
   and        pd: "pspace_distinct' s"
   and        vq: "valid_queues s"
   and       vq': "valid_queues' s"
@@ -1224,6 +1225,9 @@ proof (simp add: invs'_def valid_state'_def valid_pspace'_def
 
   show "pspace_aligned' ?s" using pa
     by (simp add: pspace_aligned'_def dom_def)
+
+  show "pspace_canonical' ?s" using pc
+    by (simp add: pspace_canonical'_def dom_def)
 
   show "pspace_distinct' ?s" using pd
     by (clarsimp simp add: pspace_distinct'_def ps_clear_def
@@ -3293,11 +3297,13 @@ lemma new_cap_object_comm_helper:
    apply clarsimp
   done
 
-crunch pspace_aligned'[wp]: updateNewFreeIndex "pspace_aligned'"
-crunch pspace_distinct'[wp]: updateNewFreeIndex "pspace_distinct'"
-crunch valid_arch_state'[wp]: updateNewFreeIndex "valid_arch_state'"
-crunch pspace_no_overlap'[wp]: updateNewFreeIndex "pspace_no_overlap' ptr n"
-crunch ctes_of[wp]: updateNewFreeIndex "\<lambda>s. P (ctes_of s)"
+crunches updateNewFreeIndex
+  for pspace_aligned'[wp]: "pspace_aligned'"
+  and pspace_distinct'[wp]: "pspace_distinct'"
+  and pspace_canonical'[wp]: "pspace_canonical'"
+  and valid_arch_state'[wp]: "valid_arch_state'"
+  and pspace_no_overlap'[wp]: "pspace_no_overlap' ptr n"
+  and ctes_of[wp]: "\<lambda>s. P (ctes_of s)"
 
 lemma updateNewFreeIndex_cte_wp_at[wp]:
   "\<lbrace>\<lambda>s. P (cte_wp_at' P' p s)\<rbrace> updateNewFreeIndex slot \<lbrace>\<lambda>rv s. P (cte_wp_at' P' p s)\<rbrace>"
@@ -4614,7 +4620,7 @@ lemma createNewObjects_def2:
     distinct dslots;
     valid_arch_state' s;
     range_cover ptr sz (Types_H.getObjectSize ty us) (length dslots);
-    ptr \<noteq> 0; sz \<le> maxUntypedSizeBits;
+    ptr \<noteq> 0; sz \<le> maxUntypedSizeBits; canonical_address (ptr && ~~ mask sz);
     ksCurDomain s \<le> maxDomain\<rbrakk>
    \<Longrightarrow> createNewObjects ty parent dslots ptr us d s =
        insertNewCaps ty parent dslots ptr us d s"
@@ -4629,6 +4635,7 @@ lemma createNewObjects_def2:
   assume extra: "y\<notin> set ys" "cte_wp_at' (\<lambda>c. cteCap c = capability.NullCap) y s"
   assume not_0: "ptr \<noteq> 0"
   assume sz_limit: "sz \<le> maxUntypedSizeBits"
+  assume ptr_cn: "canonical_address (ptr && ~~ mask sz)"
   assume kscd: "ksCurDomain s \<le> maxDomain"
   assume valid_psp: "valid_pspace' s"
   assume valid_arch_state: "valid_arch_state' s"
@@ -4644,7 +4651,7 @@ lemma createNewObjects_def2:
             insertNewCap parent slot)
         [0.e.of_nat (length ys)] (y # ys) s =
        (createNewCaps ty ptr (Suc (length ys)) us d >>= zipWithM_x (insertNewCap parent) (y # ys))  s"
-    using le list_nc dist extra range_cover not_0 sz_limit caps_reserved
+    using le list_nc dist extra range_cover not_0 sz_limit ptr_cn caps_reserved
   proof (induct ys arbitrary: y rule:rev_induct)
     case Nil
     show ?case
@@ -4738,6 +4745,7 @@ assumes check: "distinct dslots"
   and   cover: "range_cover ptr sz (Types_H.getObjectSize ty us) (length dslots)"
   and   not_0: "ptr \<noteq> 0" "length dslots \<noteq> 0"
   and sz_limit: "sz \<le> maxUntypedSizeBits"
+  and  ptr_cn: "canonical_address (ptr && ~~ mask sz)"
   and       c: "corres r P P' f (insertNewCaps ty parent dslots ptr us d)"
   and     imp: "\<And>s. P' s \<Longrightarrow> (cte_wp_at' (\<lambda>c. isUntypedCap (cteCap c)) parent s
                    \<and> (\<forall>slot \<in> set dslots. cte_wp_at' (\<lambda>c. cteCap c = capability.NullCap) slot s)
@@ -4747,7 +4755,7 @@ assumes check: "distinct dslots"
                                                           2^ (Types_H.getObjectSize ty us) - 1} s
                    \<and> valid_pspace' s \<and> valid_arch_state' s \<and> ksCurDomain s \<le> maxDomain)"
   shows "corres r P P' f (createNewObjects ty parent dslots ptr us d)"
-  using check cover not_0 sz_limit
+  using check cover not_0 sz_limit ptr_cn
   apply (clarsimp simp:corres_underlying_def)
   apply (frule imp)
   apply (frule range_cover.range_cover_le_n_less(1)[where 'a=machine_word_len, folded word_bits_def, OF _ le_refl])
@@ -4763,6 +4771,7 @@ lemma createNewObjects_wp_helper:
   assumes check: "distinct dslots"
   and   cover: "range_cover ptr sz (Types_H.getObjectSize ty us) (length dslots)"
   and   not_0: "ptr \<noteq> 0" "length dslots \<noteq> 0"
+  and  ptr_cn: "canonical_address (ptr && ~~ mask sz)"
   and   sz_limit: "sz \<le> maxUntypedSizeBits"
   shows "\<lbrace>P\<rbrace> insertNewCaps ty parent dslots ptr us d \<lbrace>Q\<rbrace>
   \<Longrightarrow> \<lbrace>P and (cte_wp_at' (\<lambda>c. isUntypedCap (cteCap c)) parent
